examples/ecAdd/proofs/gcd_props.ec
@@ -1,29 +1,23 @@
 require import Int IntDiv.
 
-op even x = ! (odd x).
 
-lemma odd_even u v : odd u => odd v => even (u - v).
+
+lemma odd_even u v : odd u => odd v => !odd (u - v).
 proof. smt(@IntDiv). qed.
 
-axiom gcd1 u v : even u => even v =>  gcd u v = 2 * gcd (u %/ 2) (v %/ 2).
-axiom gcd2 u v : even u => odd v => gcd u v = gcd (u %/ 2) v.   
+axiom gcd1 u v : !odd u => !odd v =>  gcd u v = 2 * gcd (u %/ 2) (v %/ 2).
+axiom gcd2 u v : !odd u => odd v => gcd u v = gcd (u %/ 2) v.   
 lemma gcd3 u v : gcd u v = gcd (u - v) v. smt. qed.
 lemma gcd4 u v : gcd u v = gcd v u. smt. qed.
 lemma gcd5 u v : gcd u v = gcd (-u) v. smt. qed.
 lemma gcd6 t v : gcd t v = gcd (t - v) v. smt. qed.
 
 
-
-op inv : int -> int -> int.
-axiom inv_ax u v : gcd u v = 1 => (inv u v) * v %% u = 1.
-axiom nosmt inv_ax_opp u v : gcd u v = 1 => v * (inv u v) %% u = 1. 
-
-
 op div_by2s (i : int) : int.
 axiom div_by2s1 u : 0 < u = 0 < (div_by2s u).
 axiom div_by2s2 u v : odd v => gcd (div_by2s u) v = gcd u v.
 axiom div_by2s3 u : odd (div_by2s u).
-axiom div_by2s4 u : 0 < u => even u =>  (div_by2s u) < u.
-axiom div_by2s5 u : u < 0 => even u =>  u < (div_by2s u).
-axiom div_by2s6 u : even u =>  div_by2s (u %/ 2) = div_by2s u.
+axiom div_by2s4 u : 0 < u => !odd u =>  (div_by2s u) < u.
+axiom div_by2s5 u : u < 0 => !odd u =>  u < (div_by2s u).
+axiom div_by2s6 u : !odd u =>  div_by2s (u %/ 2) = div_by2s u.
 axiom div_by2s7 u : odd u =>  div_by2s u = u.
